bst_to_list done

BSTExtra.v
@@ -1,8 +1,40 @@
 Require Import BstProject.BST.
-Require Import BstProject.BSTInsert.
 Require Import BstProject.project_lib.
 Require Import Coq.Bool.Bool.
 Require Import Coq.Arith.Arith.
+
+(* bst to list *)
+Fixpoint bst_to_list (bst: tree) : list nat :=
+  match bst with
+  | leaf => []
+  | node l v r => bst_to_list l ++ [v] ++ bst_to_list r
+end.
+
+Fixpoint list_to_bst (lst: list nat) : tree :=
+  match lst with
+  | [] => leaf
+  | head :: tail => insert head (list_to_bst tail)
+end.
+
+Example bst_lst : bst_to_list tree1 = [2;5;7;10;12;16;17].
+Proof. unfold bst_to_list. reflexivity. Qed.
+
+(* node (node (node leaf 2 leaf) 5 (node leaf 7 leaf))
+10 (* root *)
+(node (node leaf 12 leaf) 16 (node leaf 17 leaf)). *)
+
+Example lst_bst : list_to_bst [12; 17; 16; 2; 7; 5; 10]=  tree1.
+Proof. unfold list_to_bst. reflexivity. Qed.
+
+(*Useful Theorems *)
+(* Theorem bst_list_sorted : list -> bst -> list - skulle give sorted list ud
+forall t1 t2, 
+bst_to_list t1 = bst_to_list t2
+*)
+
+(* Size of list equals size of tree *)
+
+
 
 (* Exercise 3.10*)
 Fixpoint delete (x : nat) (t : tree) : tree 
